Change examples/lambda/generic_terms to better support π-calculus
In particular, allow free names to accompany GLAM constructor, rather
than forcing them to only appear with GVAR (which becomes strictly
redundant).

Fix all but π-calculus examples that depend on this tech.

examples/lambda/basics/ctermScript.sml
@@ -11,10 +11,10 @@ val tyname = "cterm"
 val vp = “(λn u:unit. n = 0)”;
 
 (* GLAM corresponds to APP, LAM and CONST *)
-val lp = “(λn (d:unit + unit + 'a) tns uns.
-             n = 0 ∧ ISL d ∧ tns = [] ∧ uns = [0;0] ∨
-             n = 0 ∧ ISR d ∧ ISL (OUTR d) ∧ tns = [0] ∧ uns = [] ∨
-             n = 0 ∧ ISR d ∧ ISR (OUTR d) ∧ tns = [] ∧ uns = [])”
+val lp = “(λn lfvs (d:unit + unit + 'a) tns uns.
+             n = 0 ∧ lfvs = 0 ∧ ISL d ∧ tns = [] ∧ uns = [0;0] ∨
+             n = 0 ∧ lfvs = 0 ∧ ISR d ∧ ISL (OUTR d) ∧ tns = [0] ∧ uns = [] ∨
+             n = 0 ∧ lfvs = 0 ∧ ISR d ∧ ISR (OUTR d) ∧ tns = [] ∧ uns = [])”
 
 val {term_ABS_pseudo11, term_REP_11, genind_term_REP, genind_exists,
      termP, absrep_id, repabs_pseudo_id, term_REP_t, term_ABS_t, newty, ...} =
@@ -25,7 +25,7 @@ val [gvar,glam] = genind_rules |> SPEC_ALL |> CONJUNCTS
 val LAM_t = mk_var("LAM", ``:string -> ^newty -> ^newty``)
 val LAM_def = new_definition(
   "LAM_def",
-  ``^LAM_t v t = ^term_ABS_t (GLAM v (INR (INL ())) [^term_REP_t t] [])``)
+  ``^LAM_t v t = ^term_ABS_t (GLAM v [] (INR (INL ())) [^term_REP_t t] [])``)
 val LAM_termP = prove(
   mk_comb(termP, LAM_def |> SPEC_ALL |> concl |> rhs |> rand),
   match_mp_tac glam >> srw_tac [][genind_term_REP]);
@@ -35,14 +35,15 @@ val APP_t = mk_var("APP", ``:^newty -> ^newty -> ^newty``)
 val APP_def = new_definition(
   "APP_def",
   ``^APP_t t1 t2 =
-       ^term_ABS_t (GLAM ARB (INL ()) [] [^term_REP_t t1; ^term_REP_t t2])``);
+       ^term_ABS_t (GLAM ARB [] (INL ()) [] [^term_REP_t t1; ^term_REP_t t2])``);
 val APP_termP = prove(
-  ``^termP (GLAM x (INL ()) [] [^term_REP_t t1; ^term_REP_t t2])``,
+  ``^termP (GLAM x [] (INL ()) [] [^term_REP_t t1; ^term_REP_t t2])``,
   match_mp_tac glam >> srw_tac [][genind_term_REP])
 val APP_t = defined_const APP_def
 
 val APP_def' = prove(
-  ``^term_ABS_t (GLAM v (INL ()) [] [^term_REP_t t1; ^term_REP_t t2]) = ^APP_t t1 t2``,
+  ``^term_ABS_t (GLAM v [] (INL ()) [] [^term_REP_t t1; ^term_REP_t t2]) =
+    ^APP_t t1 t2``,
   srw_tac [][APP_def, GLAM_NIL_EQ, term_ABS_pseudo11, APP_termP]);
 
 val VAR_t = mk_var("VAR", ``:string -> ^newty``)
@@ -57,14 +58,14 @@ val VAR_t = defined_const VAR_def
 val CONST_t = mk_var("CONST", “:'a -> ^newty”)
 val CONST_def = new_definition(
   "CONST_def",
-  “^CONST_t a = ^term_ABS_t (GLAM ARB (INR (INR a)) [][])”);
+  “^CONST_t a = ^term_ABS_t (GLAM ARB [] (INR (INR a)) [][])”);
 val CONST_termP = prove(
-  “^termP (GLAM v (INR (INR a)) [][])”,
+  “^termP (GLAM v [] (INR (INR a)) [][])”,
   srw_tac[][genind_rules]);
 val CONST_t = defined_const CONST_def
 
 val CONST_def' = prove(
-  “^term_ABS_t (GLAM v (INR (INR a)) [] []) = ^CONST_t a”,
+  “^term_ABS_t (GLAM v [] (INR (INR a)) [] []) = ^CONST_t a”,
   srw_tac[][CONST_def, GLAM_NIL_EQ, term_ABS_pseudo11, CONST_termP]);
 
 val cons_info =
@@ -155,7 +156,7 @@ val term_ind =
         |> Q.SPEC `fv`
         |> UNDISCH |> Q.SPEC `0` |> DISCH_ALL
         |> SIMP_RULE (std_ss ++ DNF_ss)
-                     [sumTheory.FORALL_SUM, supp_listpm,
+                     [sumTheory.FORALL_SUM, supp_listpm, LENGTH_NIL,
                       IN_UNION, NOT_IN_EMPTY, oneTheory.FORALL_ONE,
                       genind_exists, LIST_REL_CONS1, LIST_REL_NIL]
         |> Q.INST [`Q` |-> `λt. P (^term_ABS_t t)`]
@@ -184,8 +185,9 @@ val (_, repty) = dom_rng (type_of term_REP_t)
 val repty' = ty_antiq repty
 
 val tlf =
-  ``λ(v:string) (u:unit + unit + 'a) (ds1:(ρ -> 'r) list) (ds2:(ρ -> 'r)  list)
-                                (ts1:^repty' list) (ts2:^repty' list) (p:ρ).
+  ``λ(v:string) (fvs:string list) (u:unit + unit + 'a)
+     (ds1:(ρ -> 'r) list) (ds2:(ρ -> 'r)  list)
+     (ts1:^repty' list) (ts2:^repty' list) (p:ρ).
        if ISR u then
          if ISL (OUTR u) then tlf (HD ds1) v (cterm_ABS (HD ts1)) p: 'r
          else tcf (OUTR (OUTR u))
